

# Stochastic Calculus

## Master in Advanced Mathematics 2017-2018

Claudia Cristina Reyes Montes de Oca

### Set 3. Gaussian distributions, Gaussian processes, Brownian motion.

**Exercise 1.** (1) Show that for every  $f, g \in L^2_{a,T}$  the following identity holds:

$$\mathbb{E} \left[ \left( \int_0^T f(u) dB_u \right) \left( \int_0^T g(u) dB_u \right) \right] = \int_0^T \mathbb{E}[f(u)g(u)] du.$$

(2) Prove that if  $f : [0, T] \rightarrow \mathbb{R}$  is a deterministic continuous function, the process  $(X_t)_{t \in [0, T]}$  defined by

$$X_t := \int_0^t f(u) dB_u$$

is a zero-mean Gaussian process with independent increments.

(3) Assume that the deterministic continuous function  $f : [0, T] \rightarrow \mathbb{R}$  satisfies  $f(t) > 0$  for all  $t > 0$  and that

$$\int_0^t f^2(u) du \rightarrow T, \text{ as } t \rightarrow T.$$

For every  $t \in [0, T]$  define

$$\tau(t) := \inf \{s \in [0, T] : \int_0^s f^2(u) du \geq t\}$$

and

$$Y_t := \int_0^{\tau(t)} f(u) dB_u.$$

Prove that  $(Y_t)_{t \in [0, T]}$  is standard Brownian motion.

*Solution.* (1) Using the formula  $ab = \frac{1}{2}((a+b)^2 - a^2 - b^2)$  we get

$$\left( \int_0^T f(u) dB_u \right) \left( \int_0^T g(u) dB_u \right) = \frac{1}{2} \left[ \left( \int_0^T (f(u) + g(u)) dB_u \right)^2 - \left( \int_0^T f(u) dB_u \right)^2 - \left( \int_0^T g(u) dB_u \right)^2 \right]$$

By the Ito isometry we observe the following

$$\mathbb{E} \left[ \left( \int_0^T (f(u) + g(u)) dB_u \right)^2 \right] = \mathbb{E} \left[ \int_0^T (f(u) + g(u))^2 du \right] = \mathbb{E} \left[ \int_0^T (f^2(u) + 2f(u)g(u) + g^2(u)) du \right]$$

$$\mathbb{E} \left[ \left( \int_0^T f(u) dB_u \right)^2 \right] = \mathbb{E} \left[ \int_0^T f(u)^2 du \right]$$

$$\mathbb{E} \left[ \left( \int_0^T g(u) dB_u \right)^2 \right] = \mathbb{E} \left[ \int_0^T g(u)^2 du \right]$$

Then,

$$\frac{1}{2} \mathbb{E} \left[ \left( \int_0^T (f(u) + g(u)) dB_u \right)^2 - \left( \int_0^T f(u) dB_u \right)^2 - \left( \int_0^T g(u) dB_u \right)^2 \right] = \mathbb{E} \left[ \int_0^T f(u)g(u) du \right].$$

(2) By definition,

$$X_t = \int_0^T f(u) \mathbb{1}_{[0,t]}(u) du.$$

$t_0 < t_1 < \dots < t_n < T$ , we want

$$X_{t_1}, X_{t_2} - X_{t_1}, \dots, X_{t_n} - X_{t_{n-1}}$$

are independent. By definition, the random variables are Gaussian so the vector is Gaussian. Also,

$$\begin{aligned} \text{Cov}(X_{t_i} - X_{t_{i-1}}, X_{t_j} - X_{t_{j-1}}) &= \mathbb{E}[(X_{t_i} - X_{t_{i-1}})(X_{t_j} - X_{t_{j-1}})] \\ &= \mathbb{E}\left[\left(\int_0^T f(u) \mathbb{1}_{[t_{i-1}, t_i]}(u) dB_u\right) \left(\int_0^T f(u) \mathbb{1}_{[t_{j-1}, t_j]}(u) dB_u\right)\right] \\ &= \int_0^T \mathbb{E}[f(u)^2 \mathbb{1}_{[t_{i-1}, t_i] \cap [t_{j-1}, t_j]}] du \\ &= \int_0^T f(u)^2 \mathbb{1}_{[t_{i-1}, t_i] \cap [t_{j-1}, t_j]} du \\ &= 0 \end{aligned}$$

(3) We compute the covariance  $\text{Cov}(Y_t, Y_s)$ .

$$\begin{aligned} \text{Cov}(Y_t, Y_s) &= \mathbb{E}\left[\left(\int_0^T f(u) \mathbb{1}_{\{u \leq \tau(t)\}} dB_u\right) \left(\int_0^T f(u) \mathbb{1}_{\{u \leq \tau(s)\}} dB_u\right)\right] \\ &= \int_0^T \mathbb{E}[f(u) \mathbb{1}_{\{u \leq \tau(t)\}} f(u) \mathbb{1}_{\{u \leq \tau(s)\}}] du \\ &= \int_0^T \mathbb{E}[f^2(u) \mathbb{1}_{\{u \leq \tau(t)\}} \mathbb{1}_{\{u \leq \tau(s)\}}] du \\ &= \int_0^T \mathbb{E}[f^2(u) \mathbb{1}_{\{u \leq \tau(t)\} \cap \{u \leq \tau(s)\}}] du \\ &= \int_0^T \mathbb{E}[f^2(u) \mathbb{1}_{\{u \leq \min\{\tau(t), \tau(s)\}\}}] du \\ &= \int_0^{\min\{\tau(t), \tau(s)\}} f^2(u) du \\ &= \min\{s, t\}. \end{aligned}$$

□

**Exercise 2.** Let  $X = \int_a^b f(t)[\sin(B_t) + \cos(B_t)]dB_t$  with  $f \in L^2[a, b]$ .

- (1) Argue that the stochastic integral is well-defined.
- (2) Compute the variance of  $X$ .

*Solution.* (1)  $\int_a^b f^2(t)[\sin(B_t) + \cos(B_t)]^2 dt < \infty$

(2) We have that

$$\begin{aligned}
\text{Var}(X) &= \mathbb{E} \left[ \left( \int_a^b f(t) [\sin(B_t) + \cos(B_t)] dB_t \right)^2 \right] \\
&= \mathbb{E} \left[ \int_a^b f^2(t) [\sin(B_t) + \cos(B_t)]^2 dt \right] \\
&= \mathbb{E} \left[ \int_a^b f^2(t) [1 + 2 \cos(B_t) \sin(B_t)] dt \right] \\
&= \mathbb{E} \left[ \int_a^b f^2(t) dt + 2 \int_a^b f^2(t) \cos(B_t) \sin(B_t) dt \right] \\
&= \mathbb{E} \left[ \int_a^b f^2(t) dt \right] + 2 \mathbb{E} \left[ \int_a^b f^2(t) \cos(B_t) \sin(B_t) dt \right] \\
&= \int_a^b f^2(t) dt + 2 \int_a^b f^2(t) \mathbb{E} [\cos(B_t) \sin(B_t)] dt.
\end{aligned}$$

Now, we use the following formulas for  $\cos(x)$  and  $\sin(x)$ :

$$\cos(x) = \frac{1}{2} (e^{ix} + e^{-ix}) \quad \text{and} \quad \sin(x) = \frac{1}{2i} (e^{ix} - e^{-ix}).$$

Then,

$$\cos(x) \sin(x) = \frac{1}{4i} (e^{2ix} - e^{-2ix}).$$

Therefore,

$$\mathbb{E} [\cos(B_t) \sin(B_t)] = \frac{1}{4i} (\mathbb{E} [e^{2iB_t}] - \mathbb{E} [e^{-2iB_t}]) = 0.$$

We conclude that

$$\text{Var}(X) = \int_a^b f^2(t) dt.$$

□

**Exercise 3.** (1) Set  $X_t = \int_0^t \sqrt{s} \sin(B_s) dB_s$ ,  $t \geq 0$ . Is the stochastic integral well-defined? Compute the covariance between  $X_t$  and  $X_u$ ,  $0 \leq u \leq t$ .

(2) Let  $X_t = \int_0^t \text{sgn}(B_s) dB_s$ . Show that for  $0 \leq s < t$ ,  $X_t - X_s$  has mean zero and variance  $t - s$ .

*Solution.* (1)  $\int_0^t \mathbb{E}[s \sin^2(B_s)] ds = \frac{1}{2} \int_0^t s (e^{-2s} - 1) ds$  Compute

$$\begin{aligned}
\mathbb{E}[X_t X_u] &= \mathbb{E} \left[ \left( \int_0^t \sqrt{s} \sin(B_s) dB_s \right) \left( \int_0^u \sqrt{s} \sin(B_s) dB_s \right) \right] \\
&= \mathbb{E} \left[ \left( \int_0^t \sqrt{s} \sin(B_s) dB_s \right) \left( \int_0^t \sqrt{s} \sin(B_s) \mathbb{1}_{s \leq u} dB_s \right) \right] \\
&= \int_0^t s \mathbb{1}_{s \leq u} \mathbb{E}[\sin^2(B_s)] ds \\
&= \frac{1}{2} \int_0^u s (1 - e^{-2s}) ds \\
&= \frac{1}{4} u^2 + \frac{1}{8} (1 - (2u + 1)e^{-2u})
\end{aligned}$$

$$\sin^2(x) = -\frac{1}{4} (e^{ix} - e^{-ix})^2 = -\frac{1}{4} (e^{2ix} - 2 + e^{-2ix}) = \frac{1}{2} - \frac{1}{4} (e^{2ix} + e^{-2ix})$$

Then,

$$\mathbb{E}[\sin^2(B_s)] = \frac{1}{2} - \frac{1}{4} (\mathbb{E}[e^{2iB_s}] + \mathbb{E}[e^{-2iB_s}]) = \frac{1}{2} - \frac{1}{4} (2e^{-2s}) = \frac{1}{2} (1 - e^{-2s}).$$

(2)  $0 \leq s < t$ . Then,

$$X_t - X_s = \int_s^t \text{sgn}(B_s) dB_s$$

□

**Exercise 4.** Using the definition of the Ito integral, prove that:

- (1)  $\int_0^t s dB_s = tB_t - \int_0^t B_s ds$ .
- (2)  $\int_0^t B_s^2 dB_s = \frac{1}{3}B_t^3 - \int_0^t B_s ds$ .

*Solution.* (1)

$$\begin{aligned} \sum_i s_{t_{i-1}}(B_{t_i} - B_{t_{i-1}}) &= \sum_i (s_{t_{i-1}}B_{t_i} - s_{t_{i-1}}B_{t_{i-1}}) \\ &= \sum_i (s_{t_{i-1}}B_{t_i} - s_{t_i}B_{t_i} + s_{t_i}B_{t_i} - s_{t_{i-1}}B_{t_{i-1}}) \\ &= \sum_i (s_{t_i}B_{t_i} - s_{t_{i-1}}B_{t_{i-1}}) - \sum_i (s_{t_i} - s_{t_{i-1}}) \\ &= tB_t - \sum_i B_{t_i}(s_{t_i} - s_{t_{i-1}}). \end{aligned}$$

(2) We use the formula  $a^2(b-a) = \frac{1}{3}(b^3 - a^3 - (b-a)^3 - 3a(b-a)^2)$ .

$$\begin{aligned} \sum_i B_{t_{i-1}}^2 (B_{t_i} - B_{t_{i-1}}) &= \frac{1}{3} \sum_i \left[ (B_{t_i}^3 - B_{t_{i-1}}^3) - (B_{t_i} - B_{t_{i-1}})^3 - 3B_{t_{i-1}}(B_{t_i} - B_{t_{i-1}})^2 \right] \\ &= \frac{1}{3}B_t^3 - \frac{1}{3} \sum_i (B_{t_i} - B_{t_{i-1}})^3 - \sum_i B_{t_{i-1}}(B_{t_i} - B_{t_{i-1}})^2. \end{aligned}$$

Notice that,

$$\begin{aligned} \mathbb{E} \left[ \left( \sum_i (B_{t_i} - B_{t_{i-1}})^3 \right)^2 \right] &= \mathbb{E} \left[ \sum_i (B_{t_i} - B_{t_{i-1}})^6 \right] + 2\mathbb{E} \left[ \sum_{i,j} (B_{t_i} - B_{t_{i-1}})^3 (B_{t_j} - B_{t_{j-1}})^3 \right] \\ &= \sum_i \mathbb{E} [(B_{t_i} - B_{t_{i-1}})^6] \\ &= 15 \sum_i (t_i - t_{i-1})^3 \\ &\leq 15|\Pi^n|^2 t \rightarrow 0 \end{aligned}$$

Let us denote  $X_i := B_{t_{i-1}} ((B_{t_i} - B_{t_{i-1}})^2 - (t_i - t_{i-1}))$ . We have that

$$\mathbb{E} \left[ \left( \sum_i X_i \right)^2 \right] = \sum_i \mathbb{E}[X_i^2].$$

Indeed, for  $j < i$

$$\begin{aligned} \mathbb{E}[X_i X_j] &= \mathbb{E}[\mathbb{E}[X_i X_j \mid \mathcal{F}_{t_{j-1}}]] \\ &= \mathbb{E}[X_i B_{t_{j-1}} \mathbb{E}[(B_{t_j} - B_{t_{j-1}})^2 - (t_j - t_{j-1}) \mid \mathcal{F}_{t_{j-1}}]] \\ &= \mathbb{E}[X_i B_{t_{j-1}} (\mathbb{E}[(B_{t_j} - B_{t_{j-1}})^2] - (t_j - t_{j-1}))] \\ &= 0. \end{aligned}$$

Now,

$$\begin{aligned}
\mathbb{E}[X_i^2] &= \mathbb{E}[B_{t_{i-1}}^2 ((B_{t_i} - B_{t_{i-1}})^2 - (t_i - t_{i-1}))^2] \\
&= t_{i-1} \mathbb{E}[(B_{t_i} - B_{t_{i-1}})^2 - (t_i - t_{i-1}))^2] \\
&= t_{i-1} (\mathbb{E}[(B_{t_i} - B_{t_{i-1}})^4] - 2\mathbb{E}[(B_{t_i} - B_{t_{i-1}})^2](t_i - t_{i-1}) + (t_i - t_{i-1})^2) \\
&= t_{i-1} (3(t_i - t_{i-1})^2 - 2(t_i - t_{i-1})^2 + (t_i - t_{i-1})^2) \\
&= 2t_{i-1}(t_i - t_{i-1})^2.
\end{aligned}$$

We estimate,

$$\begin{aligned}
\mathbb{E} \left[ \left( \sum_i B_{t_{i-1}} (B_{t_i} - B_{t_{i-1}})^2 - \sum_i B_{t_{i-1}} (t_i - t_{i-1}) \right)^2 \right] &= \mathbb{E} \left[ \left( \sum_i B_{t_{i-1}} ((B_{t_i} - B_{t_{i-1}})^2 - (t_i - t_{i-1})) \right)^2 \right] \\
&= \mathbb{E} \left[ \left( \sum_i X_i \right)^2 \right] \\
&= \sum_i \mathbb{E}[X_i^2] \\
&= 2 \sum_i t_{i-1} (t_i - t_{i-1})^2 \\
&\leq 2|\Pi^n| t^2 \rightarrow 0
\end{aligned}$$

□

**Exercise 5.** Let  $u \in L_{a,T}^2$ . Prove that the process

$$\left( \int_0^t u_s dB_s \right)^2 - \int_0^t u_s^2 ds, \quad t \in [0, T],$$

is a martingale.

*Solution.*

□

**Exercise 6.** Prove that the following stochastic processes are martingales with respect to the natural filtration of the Brownian motion.

- (1)  $M_t = B_t^3 - 3tB_t, t \geq 0;$
- (2)  $X_t = \exp\left(\frac{1}{2}t\right) \cos(B_t), t \geq 0;$
- (3)  $X_t = (B_t + t) \exp\left(-B_t - \frac{1}{2}t\right).$

*Solution.* (1) We use the items (1) and (2) in Problem 4 and we write

$$\begin{aligned}
M_t &= 3 \left( \int_0^t B_s^2 dB_s + \int_0^t B_s ds - \int_0^t s dB_s - \int_0^t B_s ds \right) \\
&= \int_0^t 3(B_s^2 - s) dB_s.
\end{aligned}$$

(2) We consider the function

$$\begin{aligned}
f &: [0, T] \times \mathbb{R} \rightarrow \mathbb{R} \\
(t, x) &\mapsto \exp\left(\frac{1}{2}t\right) \cos(x).
\end{aligned}$$

$$\partial_t f(t, x) = \frac{1}{2} \exp\left(\frac{1}{2}t\right) \cos(x).$$

$$\partial_x f(t, x) = -\exp\left(\frac{1}{2}t\right) \sin(x).$$

$$\partial_{xx}^2 f(t, x) = -\exp\left(\frac{1}{2}t\right) \cos(x).$$

Applying the Ito formula we obtain

$$\begin{aligned} X_t &= f(0, B_0) + \int_0^t \frac{1}{2} \exp\left(\frac{1}{2}s\right) \cos(B_s) ds - \int_0^t \exp\left(\frac{1}{2}s\right) \sin(B_s) dB_s - \frac{1}{2} \int_0^t \exp\left(\frac{1}{2}s\right) \cos(B_s) ds \\ &= 1 - \int_0^t \exp\left(\frac{1}{2}s\right) \sin(B_s) dB_s. \end{aligned}$$

(3) We consider the function

$$f : [0, T] \times \mathbb{R} \rightarrow \mathbb{R}$$

$$(t, x) \mapsto (x + t) \exp\left(-x - \frac{1}{2}t\right).$$

$$\partial_t f(t, x) = -\frac{1}{2}(x + t) \exp\left(-x - \frac{1}{2}t\right) + \exp\left(-x - \frac{1}{2}t\right) = \exp\left(-x - \frac{1}{2}t\right) \left(1 - \frac{1}{2}(x + t)\right)$$

$$\partial_x f(t, x) = -(x + t) \exp\left(-x - \frac{1}{2}t\right) + \exp\left(-x - \frac{1}{2}t\right) = \exp\left(-x - \frac{1}{2}t\right) (1 - (x + t))$$

$$\partial_{xx}^2 f(t, x) = -(1 - (x + t)) \exp\left(-x - \frac{1}{2}t\right) - \exp\left(-x - \frac{1}{2}t\right) = -\exp\left(-x - \frac{1}{2}t\right) (2 - x - t).$$

Applying the Ito formula we obtain

$$\begin{aligned} X_t &= \int_0^t \exp\left(-B_s - \frac{1}{2}s\right) \left(1 - \frac{1}{2}(B_s + s)\right) ds + \int_0^t \exp\left(-B_s - \frac{1}{2}s\right) (1 - (B_s + s)) dB_s \\ &\quad - \frac{1}{2} \int_0^t \exp\left(-B_s - \frac{1}{2}s\right) (2 - B_s - s) ds \\ &= \int_0^t \exp\left(-B_s - \frac{1}{2}s\right) (1 - (B_s + s)) dB_s. \end{aligned}$$

□

**Exercise 7.** Write the Ito differential of the following processes.

- (1)  $X_t = 2 + t + \exp(B_t)$ ;
- (2)  $X_t = B_t^2$ ;
- (3)  $X_t = (t + \lambda, B_t)$ , where  $\lambda > 0$  is a constant;
- (4)  $X_t = B_1^2(t) + B_2^2(t)$ , where  $\{(B_1(t), B_2(t)), t \geq 0\}$  is a 2-dimensional Brownian motion;
- (5)  $X_t = (B_1(t) + B_2(t) + B_3(t), B_2(t)^2 - B_1(t)B_3(t))$ , where  $\{(B_1(t), B_2(t), B_3(t)), t \geq 0\}$  is a 3-dimensional Brownian motion.
- (6)  $X_t = \exp\left(\alpha_0 t + \sum_{j=1}^n \alpha_j B_j(t)\right)$ , where  $\{(B_1(t), \dots, B_n(t)), t \geq 0\}$  is an  $n$ -dimensional Brownian motion, and  $\alpha_0, \dots, \alpha_n \in \mathbb{R}$  are some constants.

*Solution.* (1) We consider the function

$$f : [0, T] \times \mathbb{R} \rightarrow \mathbb{R}$$

$$(t, x) \mapsto 2 + t + \exp(x).$$

$$\partial_t f(t, x) = 1.$$

$$\partial_x f(t, x) = \exp(x).$$

$$\partial_{xx}^2 f(t, x) = \exp(x).$$

Ito:

$$X_t = 3 + \int_0^t ds + \int_0^t \exp(B_s) dB_s + \frac{1}{2} \int_0^t \exp(B_s) ds$$

Then,

$$dX_t = \left(1 + \frac{1}{2} \exp(B_t)\right) dt + \exp(B_t) dB_t.$$

(2) We consider the function

$$\begin{aligned} f : [0, T] \times \mathbb{R} &\rightarrow \mathbb{R} \\ (t, x) &\mapsto x^2. \end{aligned}$$

$$\partial_t f(t, x) = 0.$$

$$\partial_x f(t, x) = 2x.$$

$$\partial_{xx}^2 f(t, x) = 2.$$

Ito:

$$X_t = \int_0^t 2B_s dB_s + \frac{1}{2} \int_0^t 2ds$$

Then,

$$dX_t = 2B_t dB_t + dt.$$

(3) In this case, we have

$$dX_t = \begin{pmatrix} dt \\ dB_t \end{pmatrix} = \begin{pmatrix} 1 \\ 0 \end{pmatrix} dt + \begin{pmatrix} 0 \\ 1 \end{pmatrix} dB_t.$$

(4) We consider the function

$$\begin{aligned} f : [0, T] \times \mathbb{R}^2 &\rightarrow \mathbb{R} \\ (t, x, y) &\mapsto x^2 + y^2. \end{aligned}$$

$$\partial_t f(t, x, y) = 0.$$

$$\partial_x f(t, x, y) = 2x.$$

$$\partial_y f(t, x, y) = 2y.$$

$$\partial_{xy} f(t, x, y) = 0 = \partial_{yx} f(t, x, y).$$

$$\partial_{xx}^2 f(t, x, y) = 2 = \partial_{yy}^2 f(t, x, y).$$

Ito:

$$\begin{aligned} X_t &= \int_0^t 2B_1(s) dB_1(s) + \int_0^t 2B_2(s) dB_2(s) + \frac{1}{2} \int_0^t 2dB_1(s) dB_1(s) + \frac{1}{2} \int_0^t 2dB_2(s) dB_2(s) \\ &= \int_0^t 2B_1(s) dB_1(s) + \int_0^t 2B_2(s) dB_2(s) + \int_0^t ds + \int_0^t ds \end{aligned}$$

Then,

$$dX_t = 2B_1(t) dB_1(t) + 2B_2(t) dB_2(t) + 2dt.$$

(5) We consider the following function

$$\begin{aligned} f_1 : [0, T] \times \mathbb{R}^3 &\rightarrow \mathbb{R} \\ (t, x_1, x_2, x_3) &\mapsto x_1 + x_2 + x_3 \end{aligned}$$

and

$$f_2 : [0, T] \times \mathbb{R}^3 \rightarrow \mathbb{R}$$

$$(t, x, y, z) \mapsto y^2 - xz.$$

For  $f_1$ , the derivatives

$$\partial_t f(t, x_1, x_2, x_3) = 0.$$

$$\partial_{x_i} f(t, x_1, x_2, x_3) = 1 \text{ for } i = 1, \dots, 3.$$

$$\partial_{x_k x_l}^2 f(t, x_1, x_2, x_3) = 0 \text{ for all } k, l = 1, \dots, 3.$$

Ito:

$$f_1(t, B_1(t), B_2(t), B_3(t)) = \int_0^t dB_1(s) + \int_0^t dB_2(s) + \int_0^t dB_3(s).$$

Then,

$$df_1(t, B_1(t), B_2(t), B_3(t)) = dB_1(t) + dB_2(t) + dB_3(t).$$

Now, consider the following function

$$f_1 : [0, T] \times \mathbb{R}^3 \rightarrow \mathbb{R}$$

$$(t, x_1, x_2, x_3) \mapsto x_2^2 - x_1 x_3$$

For  $f_2$ , the derivatives

$$\partial_t f(t, x_1, x_2, x_3) = 0.$$

$$\partial_{x_1} f(t, x_1, x_2, x_3) = -x_3.$$

$$\partial_{x_2} f(t, x_1, x_2, x_3) = 2x_2.$$

$$\partial_{x_3} f(t, x_1, x_2, x_3) = -x_1.$$

$$\partial_{x_k x_k}^2 f(t, x_1, x_2, x_3) = 0 \text{ for } k \neq 2 \text{ and } \partial_{x_2 x_2}^2 f(t, x_1, x_2, x_3) = 2.$$

$$\partial_{x_1 x_3}^2 f(t, x_1, x_2, x_3) = \partial_{x_1 x_3}^2 f(t, x_1, x_2, x_3) = -1$$

$$\partial_{x_1 x_2} f(t, x_1, x_2, x_3) = \partial_{x_2 x_3} f(t, x_1, x_2, x_3) = \partial_{x_3 x_2} f(t, x_1, x_2, x_3) = \partial_{x_2 x_3} f(t, x_1, x_2, x_3) = 0$$

Ito:

$$\begin{aligned} f_2(t, B_1(t), B_2(t), B_3(t)) &= \int_0^t -B_3(s)dB_1(s) + \int_0^t 2B_2(s)dB_2(s) + \int_0^t -B_1(s)dB_3(s) \\ &\quad + \frac{1}{2} \int_0^t 2dB_2(s)dB_2(s) + \frac{1}{2} \int_0^t -dB_1(s)dB_3(s) + \frac{1}{2} \int_0^t -dB_3(s)dB_1(s) \\ &= \int_0^t -B_3(s)dB_1(s) + \int_0^t 2B_2(s)dB_2(s) + \int_0^t -B_1(s)dB_3(s) \\ &\quad + \int_0^t ds. \end{aligned}$$

Then,

$$df_2(t, B_1(t), B_2(t), B_3(t)) = dt - B_3(t)dB_1(t) + 2B_2(t)dB_2(t) - B_1(t)dB_3(t).$$

Finally,

$$\begin{aligned} dX_t &= (df_1(t, B_1(t), B_2(t), B_3(t)), df_2(t, B_1(t), B_2(t), B_3(t))) \\ &= (dB_1(t) + dB_2(t) + dB_3(t), dt - B_3(t)dB_1(t) + 2B_2(t)dB_2(t) - B_1(t)dB_3(t)) \end{aligned}$$

$$\text{or } dX_t = \begin{pmatrix} 0 \\ 1 \end{pmatrix} dt + \begin{pmatrix} 1 & 1 & 1 \\ -B_3(t) & 2B_2(t) & -B_1(t) \end{pmatrix} \begin{pmatrix} dB_1(t) \\ dB_2(t) \\ dB_3(t) \end{pmatrix}$$



(6) Now, consider the following function. For  $\alpha_0, \dots, \alpha_n \in \mathbb{R}$  some constants.

$$f : [0, T] \times \mathbb{R}^n \rightarrow \mathbb{R}$$

$$(t, x_1, \dots, x_n) \mapsto \exp \left( \alpha_0 t + \sum_{j=1}^n \alpha_j x_j \right)$$

$$\partial_t f(t, x_1, \dots, x_n) = \alpha_0 \exp \left( \alpha_0 t + \sum_{j=1}^n \alpha_j x_j \right).$$

$$\partial_{x_j} f(t, x_1, \dots, x_n) = \alpha_j \exp \left( \alpha_0 t + \sum_{j=1}^n \alpha_j x_j \right).$$

$$\partial_{x_j x_j}^2 f(t, x_1, \dots, x_n) = \alpha_j^2 \exp \left( \alpha_0 t + \sum_{j=1}^n \alpha_j x_j \right).$$

$$\partial_{x_j x_l} f(t, x_1, \dots, x_n) = \partial_{x_l x_j} f(t, x_1, \dots, x_n) = \alpha_j \alpha_l \exp \left( \alpha_0 t + \sum_{j=1}^n \alpha_j x_j \right).$$

Ito,

$$\begin{aligned} X_t &= 1 + \int_0^t \alpha_0 \exp \left( \alpha_0 s + \sum_{j=1}^n \alpha_j B_j(s) \right) ds + \sum_{j=1}^n \int_0^t \alpha_j \exp \left( \alpha_0 s + \sum_{j=1}^n \alpha_j B_j(s) \right) dB_j(s) \\ &\quad + \frac{1}{2} \sum_{j=1}^n \int_0^t \alpha_j^2 \exp \left( \alpha_0 s + \sum_{j=1}^n \alpha_j B_j(s) \right) dB_j(s) dB_j(s) \\ &\quad + \frac{1}{2} \sum_{j \neq l} \int_0^t \alpha_j \alpha_l \exp \left( \alpha_0 s + \sum_{j=1}^n \alpha_j B_j(s) \right) dB_j(s) dB_l(s) \\ &= 1 + \int_0^t \alpha_0 \exp \left( \alpha_0 s + \sum_{j=1}^n \alpha_j B_j(s) \right) ds + \sum_{j=1}^n \int_0^t \alpha_j \exp \left( \alpha_0 s + \sum_{j=1}^n \alpha_j B_j(s) \right) dB_j(s) \\ &\quad + \frac{1}{2} \sum_{j=1}^n \int_0^t \alpha_j^2 \exp \left( \alpha_0 s + \sum_{j=1}^n \alpha_j B_j(s) \right) ds \\ &= 1 + \int_0^t \alpha_0 X_s ds + \sum_{j=1}^n \int_0^t \alpha_j X_s dB_j(s) + \frac{1}{2} \sum_{j=1}^n \int_0^t \alpha_j^2 X_s ds \\ &= 1 + \int_0^t \left( \alpha_0 + \frac{1}{2} \sum_{j=1}^n \alpha_j^2 \right) X_s ds + \int_0^t X_s \sum_{j=1}^n \alpha_j dB_j. \end{aligned}$$

Therefore,

$$dX_t = \left( \alpha_0 + \frac{1}{2} \sum_{j=1}^n \alpha_j^2 \right) X_t dt + X_t \left( \sum_{j=1}^n \alpha_j dB_j \right).$$

□

**Exercise 8.** Consider two positive Ito processes:

$$dX_t^{(i)} = X_t^{(i)} \left( \alpha_t^{(i)} dt + \beta_t^{(i)} dB_t \right), \quad i = 1, 2$$

Find the Ito differential of the log-ratio process

$$Y_t := \ln \left( \frac{X_t^{(1)}}{X_t^{(2)}} \right), \quad t \geq 0.$$

*Solution.* Consider the function  $f(x, y) = \ln \left( \frac{x}{y} \right)$ . Then,

$$\begin{aligned} \partial_x f(x, y) &= \frac{1}{x} & \partial_{xx} f(x, y) &= -\frac{1}{x^2}; \\ \partial_y f(x, y) &= -\frac{1}{y} & \partial_{yy} f(x, y) &= \frac{1}{y^2}; \\ \partial_{xy} f(x, y) &= 0 & \partial_{yx} f(x, y) &= 0. \end{aligned}$$

$$\begin{aligned} dX_t^{(i)} dX_t^{(i)} &= (X_t^{(i)})^2 \left( \alpha_t^{(i)} dt + \beta_t^{(i)} dB_t \right)^2 \\ &= (X_t^{(i)})^2 \left( (\alpha_t^{(i)})^2 dt + 2\alpha_t^{(i)} \beta_t^{(i)} dt dB_t + (\beta_t^{(i)})^2 dB_t dB_t \right) \\ &= (X_t^{(i)})^2 (\beta_t^{(i)})^2 dt. \end{aligned}$$

Ito:

$$\begin{aligned} Y_t &= c + \int_0^t \frac{1}{X_s^{(1)}} dX_s^{(1)} + \int_0^t -\frac{1}{X_s^{(2)}} dX_s^{(2)} + \frac{1}{2} \left( \int_0^t -\frac{1}{(X_s^{(1)})^2} dX_s^{(1)} dX_s^{(1)} + \int_0^t \frac{1}{(X_s^{(2)})^2} dX_s^{(2)} dX_s^{(2)} \right) \\ &= c + \int_0^t \left( \alpha_s^{(1)} ds + \beta_s^{(1)} dB_s \right) + \int_0^t -\left( \alpha_s^{(2)} ds + \beta_s^{(2)} dB_s \right) + \frac{1}{2} \left( \int_0^t -(\beta_s^{(1)})^2 ds + \int_0^t (\beta_s^{(2)})^2 ds \right) \\ &= c + \int_0^t \left( \alpha_s^{(1)} - \alpha_s^{(2)} - \frac{1}{2} \beta_s^{(1)} + \frac{1}{2} \beta_s^{(2)} \right) ds + \int_0^t \left( \beta_s^{(1)} - \beta_s^{(2)} \right) dB_s \end{aligned}$$

Thus, we get

$$dY_t = bt + adB_t$$

where

$$b = \alpha_s^{(1)} - \alpha_s^{(2)} - \frac{1}{2} \beta_s^{(1)} + \frac{1}{2} \beta_s^{(2)} \quad \text{and} \quad a = \beta_s^{(1)} - \beta_s^{(2)}.$$

□

**Exercise 9.**  $\{B_t, t \geq 0\}$  is a Brownian motion and  $f : (0, \infty) \times \mathbb{R} \rightarrow \mathbb{R}$  is continuous, continuous differentiable in the first argument and twice continuously differentiable in the second argument ( $f \in \mathcal{C}^{1,2}(\mathbb{R}) \cap \mathcal{C}(\mathbb{R})$ ). Moreover, we assume that

$$\sup_{(x,t) \in (0,\infty) \times \mathbb{R}} |f(t, x)| + |\partial_t f(t, x)| + |\partial_x f(t, x)| + |\partial_{xx}^2 f(t, x)| < \infty.$$

Prove that the process

$$M_t^f := f(t, B_t) - f(0, 0) - \int_0^t \mathcal{L}f(s, B_s) ds, \quad t \geq 0,$$

is a martingale with respect to the filtration generated by the Brownian motion, where

$$\mathcal{L} = \partial_t + \frac{1}{2} \partial_{xx}^2.$$

*Solution.* We can apply Ito

$$\begin{aligned} f(t, B_t) &= f(0, 0) + \int_0^t \partial_s f(s, B_s) ds + \int_0^t \partial_x f(s, B_s) dB_s + \frac{1}{2} \int_0^t \partial_{xx}^2 f(s, B_s) ds \\ &= f(0, 0) + \int_0^t \mathcal{L}f(s, B_s) ds + \int_0^t \partial_x f(s, B_s) dB_s. \end{aligned}$$

Thus,

$$M_t^f = \int_0^t \partial_x f(s, B_s) dB_s.$$

□

**Exercise 10.**  $\{B_t, t \geq 0\}$  is a Brownian motion,  $\Phi \in C_b^2(\mathbb{R})$  (twice continuously differentiable,  $\Phi$  and its derivatives up to the second order are bounded),  $\Phi(0) = 0$ ,  $f, g \in L_{a,T}^2$ . Prove that

$$\begin{aligned} \mathbb{E} \left[ \left( \int_0^t f(s) dB_s \right) \left( \Phi \left( \int_0^t g(s) dB_s \right) \right) \right] &= \mathbb{E} \left[ \int_0^t f(s) g(s) \Phi' \left( \int_0^s g(r) dB_r \right) ds \right] \\ &\quad + \frac{1}{2} \mathbb{E} \left[ \int_0^t \left( \int_0^s f(r) dB_r \right) \Phi'' \left( \int_0^s g(\alpha) dB_\alpha \right) g^2(s) ds \right]. \end{aligned}$$

*Solution.* Consider the following Ito processes:

$$X_t = \int_0^t f(s) dB_s \quad \text{and} \quad Y_t = \int_0^t g(s) dB_s.$$

By hypothesis, we can apply Itos formula to  $\Phi(Y_t)$  to obtain

$$\begin{aligned} \Phi(Y_t) &= \Phi(Y_0) + \int_0^t \Phi'(Y_s) ds + \frac{1}{2} \int_0^t \Phi''(Y_s) ds \\ &= \int_0^t \Phi'(Y_s) g(s) dB_s + \frac{1}{2} \int_0^t \Phi''(Y_s) g^2(s) ds. \end{aligned}$$

In differential form,

$$d\Phi(Y_t) = \Phi'(Y_t) g(t) dB_t + \frac{1}{2} \Phi''(Y_t) g^2(t) dt.$$

Thus,  $\Phi(Y_s)$  is an Ito process with  $u_t = \Phi'(Y_t) g(t)$  and  $v_t = \frac{1}{2} \Phi''(Y_t) g^2(t)$ . By the integration by parts formula,

$$\begin{aligned} X_t \Phi(Y_t) &= \left( \int_0^t f(s) dB_s \right) \left( \Phi \left( \int_0^t g(s) dB_s \right) \right) \\ &= \int_0^t X_s d\phi(Y_s) + \int_0^t \Phi(Y_s) dX_s + \int_0^t \Phi'(Y_s) g(s) f(s) ds \\ &= \int_0^t X_s \Phi'(Y_s) g(s) dB_s + \frac{1}{2} \int_0^t X_s \Phi''(Y_s) g^2(s) ds + \int_0^t \Phi(Y_s) f(s) dB_s + \int_0^t \Phi'(Y_s) g(s) f(s) ds. \end{aligned}$$

Therefore,

$$\mathbb{E} [X_t \Phi(Y_t)] = \mathbb{E} \left[ \int_0^t \Phi'(Y_s) g(s) f(s) ds \right] + \frac{1}{2} \mathbb{E} \left[ \int_0^t X_s \Phi''(Y_s) g^2(s) ds \right]$$

□